\begin{equation*}
    \setlength{\jot}{\baselineskip}
    \begin{split}
        \log\left(\frac{\sigma(x)}{1-\sigma(x)}\right) &= \log\left(\frac{\frac{e^x}{e^x+1}}{1-\frac{e^x}{e^x+1}}\right) \\ &=
        \log\left(\frac{e^x}{(e^x+1)\left(1-\frac{e^x}{e^x+1}\right)}\right) \\ &=
        \log\left(\frac{e^x}{e^x-\frac{e^x}{e^x+1}-\frac{e^{2x}}{e^x+1}+1}\right) \\ &=
        \log\left(\frac{e^x}{\frac{e^{2x}+e^x-e^x-e^{2x}+e^x+1}{e^x+1}}\right) \\ &=
        \log\left(\frac{e^x}{\frac{e^x+1}{e^x+1}}\right) = \log(e^x) = x
    \end{split}
\end{equation*}